temp

src/tactic/zify.lean
@@ -24,15 +24,16 @@ open tactic
 
 namespace zify
 
-@[user_attribute]
+mk_simp_attribute zify ""
+/- @[user_attribute]
 meta def zify_attr : user_attribute unit unit :=
 { name := `zify,
-  descr := "",
+  descr := ""/- ,
   after_set := some $ λ n _ _, do
     d ← get_decl n,
     guard (d.type = `(expr → tactic  (expr × expr)))
-      <|> fail "zify patterns must have type `expr → tactic (expr × expr)`" }
-
+      <|> fail "zify patterns must have type `expr → tactic (expr × expr)`" -/ } -/
+/-
 /-- Returns a list of all `zify` patterns in the context. -/
 meta def get_patterns : tactic (list (expr → tactic  (expr × expr))) :=
 attribute.get_instances `zify >>= mmap (λ t, mk_const t >>= eval_expr (expr → tactic (expr × expr)))
@@ -50,7 +51,15 @@ meta def comparison : expr → tactic (expr × expr)
 | `(@ge ℕ %%_ %%lhs %%rhs) := mk_app_tuple ``int.coe_nat_le_coe_nat_iff rhs lhs ``((%%lhs : ℤ) ≥ %%rhs)
 | `(@gt ℕ %%_ %%lhs %%rhs) := mk_app_tuple ``int.coe_nat_lt_coe_nat_iff rhs lhs ``((%%lhs : ℤ) > %%rhs)
 | `(@eq ℕ %%lhs %%rhs) := mk_app_tuple ``int.coe_nat_eq_coe_nat_iff lhs rhs ``((%%lhs : ℤ) = %%rhs)
-| _ := failed
+| _ := failed -/
+
+meta def lift_to_z (e : expr) : tactic (expr × expr) :=
+do ns ← attribute.get_instances `zify >>= mmap (λ n, do c ← mk_const n, return (c, tt)),
+   sl ← simp_lemmas.mk.append_with_symm ns,
+   simplify sl [] e
+
+
+attribute [zify] int.coe_nat_le_coe_nat_iff int.coe_nat_lt_coe_nat_iff int.coe_nat_eq_coe_nat_iff
 
 
 end zify
@@ -60,15 +69,22 @@ Given `e` a proposition about natural numbers,
 `zify e` tries to translate it to a proposition `e'` about integers.
 Returns `e'` and a proof that `e = e'`. -/
 meta def tactic.zify1 (e : expr) : tactic (expr × expr) :=
-do zify_patterns ← zify.get_patterns,
-   (zv, iff_pf) ← zify_patterns.mfirst (λ f, f e),
+do --zify_patterns ← zify.get_patterns,
+  --  trace "1",
+  --  (zv, iff_pf) ← zify.lift_to_z e <|> fail "failed to lift to ℤ", --zify_patterns.mfirst (λ f, f e),
+  --  trace zv,
    (s, _) ← mk_simp_set tt [`push_cast] [],
-   (newe, cast_eq) ← simplify (s.erase [`int.coe_nat_succ]) [] zv {fail_if_unchanged := ff},
-   pex_pf ← mk_app `propext [iff_pf] >>= mk_eq_symm,
-   prod.mk newe <$> mk_eq_trans pex_pf cast_eq
+  --  (newe, cast_eq) ← simplify (s.erase [`int.coe_nat_succ]) [] e {fail_if_unchanged := ff},
+  --  --pex_pf ← mk_app `propext [iff_pf] >>= mk_eq_symm,
+  --  prod.mk newe <$> mk_eq_trans pex_pf cast_eq
+  simplify (s.erase [`int.coe_nat_succ]) [] e {fail_if_unchanged := ff}
 
 meta def tactic.zify : expr → tactic (expr × expr) := λ z,
-prod.snd <$> simplify_bottom_up () (λ _ e, prod.mk () <$> tactic.zify1 e) z
+do ((), z1, p1) ← simplify_bottom_up () (λ _ e, prod.mk () <$> zify.lift_to_z e) z,
+trace "1", trace z1,
+   ((), z2, p2) ← simplify_bottom_up () (λ _ e, prod.mk () <$> tactic.zify1 e) z1 {fail_if_unchanged := ff},
+   trace "2",
+   prod.mk z2 <$> mk_eq_trans p1 p2
 
 /--
 Given `h` a proof of a proposition about natural numbers,
@@ -87,15 +103,14 @@ do locs ← l.get_locals,
 replace_at tactic.zify locs l.include_goal >>= guardb
 
 end
-
-example (a b c x y z : ℕ) (h : ¬ x*y*z < 0) : a + 3*b > c :=
+example (a b c x y z : ℕ) (h : ¬ x*y*z < 0) : a + 3*b < c :=
 begin
+  simp only with zify,
   zify at h ⊢,
   guard_hyp h := ¬↑x * ↑y * ↑z < (0 : ℤ),
-  guard_target ↑a + 3 * ↑b > (↑c : ℤ),
+  guard_target (↑a : ℤ) + 3 * ↑b > ↑c,
   admit
 end
-
 
 example (a b : ℕ) : a ≤ b :=
 begin
